Valaig/Transform/Unroll.lean
@@ -8,6 +8,7 @@ open Aig
 
 namespace unroll
 
+@[expose]
 def assignMap (assign : LeafIdx -> Frame -> Bool) (map : Std.HashMap InputIdx InputIdx) : LeafIdx -> Frame -> Bool
 | .input idx, frame =>
   match map.get? idx with
@@ -21,7 +22,7 @@ private def walker (old : WFAig) : old.CachingForwardsWalker (WFAig × Std.HashM
   cacheMotive state size le sm var lt lit :=
     ∃ (h : lit.validIn state.fst),
       ∀ {assign},
-        ⟦old, var, 1, assign⟧sv = ⟦state.fst, lit, 0, assignMap assign state.snd⟧s
+        ⟦old, var, assign⟧cv1 = ⟦state.fst, lit, assignMap assign state.snd⟧c0
 
   init := ⟨old, .emptyWithCapacity old.numInputs⟩
   initState := by grind
@@ -49,10 +50,10 @@ private def walker (old : WFAig) : old.CachingForwardsWalker (WFAig × Std.HashM
     · simp; grind
     next idx =>
       simp only [WFAig.raw_fst_addInput, WFAig.snd_addInput, snd_addInput]
-      rw [denoteS_mono (mono_addInput (aig := state.fst))]
+      rw [denoteC_mono (mono_addInput (aig := state.fst))]
       · rcases cm hvar with ⟨_, cm⟩
         rw [cm]
-        apply denoteS_of_assign_eq (wf := by grind)
+        apply denoteC_of_assign_eq (wf := by grind)
         grind [assignMap]
       all_goals grind
     · simp; grind
@@ -66,11 +67,11 @@ private def walker (old : WFAig) : old.CachingForwardsWalker (WFAig × Std.HashM
     · simp; grind [assignMap]
     next idx heq =>
       have : old.nodes[var] = Node.latch idx := by grind
-      simp only [denoteSV_getElem_nodes_latch this, getNext_eq]
+      simp only [denoteCV_getElem_nodes_latch this, getNext_eq]
       have : state.fst.latches[idx] = old.latches[idx] := by grind
-      rw [denoteS_mono sm.left (lit := state.fst.latches[idx].next)]
+      rw [denoteC_mono sm.left (lit := state.fst.latches[idx].next)]
       · rw [Data.AbsMap.getElem_mono (mono_latches_mono sm.left)]
-        · apply denoteS_of_assign_eq (wf := by grind)
+        · apply denoteC_of_assign_eq (wf := by grind)
           grind [assignMap]
         · grind
       all_goals grind
@@ -83,34 +84,39 @@ end unroll
 
   TODO: Strashing whilst unrolling
 -/
-def unroll (aig : WFAig) : WFAig × Data.VarCache Lit :=
+def unroll (aig : WFAig) : WFAig × Data.VarCache Lit × Std.HashMap InputIdx InputIdx :=
   let res := (unroll.walker aig).walk
-  (res.fst.fst, res.snd)
+  (res.fst.fst, res.snd, res.fst.snd)
 
-@[simp, grind .]
-theorem mono_unroll {aig : WFAig} :
+@[simp, grind! .]
+theorem mono_unroll (aig : WFAig) :
     aig ≤ (unroll aig).fst := by
   have := (unroll.walker aig).stateMotive_walk
   grind [unroll, unroll.walker]
 
 @[simp, grind .]
 theorem size_cache_unroll {aig : WFAig} :
-    (unroll aig).snd.size = aig.size := by
+    (unroll aig).snd.fst.size = aig.size := by
   have := (unroll.walker aig).stateMotive_walk
   grind [unroll, unroll.walker]
 
 @[simp, grind .]
-theorem mem_nodes_unroll {aig : WFAig} {var : Var} (mem : var ∈ aig.nodes) :
-    var ∈ (unroll aig).fst.nodes := by
-  have := (unroll.walker aig).stateMotive_walk
+theorem mem_nodes_unroll_of_mem_cache {aig : WFAig} {var : Var} h :
+    ((unroll aig).snd.fst[var]'h).var ∈ (unroll aig).fst.nodes := by
+  have := (unroll.walker aig).cacheMotive_walk
   grind [unroll, unroll.walker]
 
+@[simp, grind =]
 theorem denote_unroll {assign} {aig : WFAig} {var : Var} mem :
-  ∃ assign',
-    ⟦aig, var, 1, assign⟧sv =
-      ⟦(unroll aig).fst, (unroll aig).snd[var]'mem, assign'⟧s0 := by
+    ⟦(unroll aig).fst, (unroll aig).snd.fst[var]'mem, unroll.assignMap assign (unroll aig).snd.snd⟧c0 =
+      ⟦aig, var, assign⟧cv1 := by
   have := (unroll.walker aig).cacheMotive_walk var (by grind)
-  exists unroll.assignMap assign (unroll.walker aig).walk.fst.snd
+  grind [unroll, unroll.walker]
+
+@[simp, grind .]
+theorem unroll_not_mem_of_mem_inputs {aig : WFAig} {idx : InputIdx} (mem : idx ∈ aig.inputs) :
+    idx ∉ (unroll aig).snd.snd := by
+  have := (unroll.walker aig).stateMotive_walk
   grind [unroll, unroll.walker]
 
 end Valaig.Transform
