Valaig/External/Cert.lean
@@ -1,3 +1,4 @@
 module
 
 public import Valaig.External.Cert.Basic
+public import Valaig.External.Cert.Product
